refactoring pt1

src/Framework/Annotate.v
@@ -1,121 +1,531 @@
-From CertiCoq.LambdaANF Require Import Ensembles_util.
+From Coq Require Import ZArith.ZArith Sets.Ensembles Lists.List.
+From CertiCoq.LambdaANF Require Import Ensembles_util map_util set_util List_util tactics.
+Import ListNotations.
+Require Import Lia.
+From Hammer Require Import Hammer Tactics Reflect.
+
 From Framework Require Import Util ANF0 ANF Refl0 Refl Erase.
 
 Module A0 := ANF0.
 Module A1 := ANF.
 
-Module Type Annotate.
+Module AnnotateUtil.
 
-  (* Analysis result type *)
-  Parameter web_map : Type.
+  Lemma V_mono_Forall_aux :
+    forall i j V vs1 vs2,
+      (forall k : nat,
+          k < S i ->
+          forall (j : nat) (v1 : A0.val) (v2 : A1.wval), V k v1 v2 -> j <= k -> V j v1 v2) ->
+      Forall2 (V i) vs1 vs2 ->
+      j <= i ->
+      Forall2 (V j) vs1 vs2.
+  Proof.
+    intros.
+    revert vs2 H0.
+    induction vs1; intros; inv H0; auto.
+    rename l' into vs2.
+    constructor; auto.
+    eapply H; eauto; lia.
+  Qed.
 
-  (* Analysis result invariant used by transformation *)
-  Parameter web_map_inv : web_map -> Prop.
+  Lemma V_mono_Forall_mono (V : nat -> A0.val -> A1.wval -> Prop) :
+    (forall i j v1 v2, V i v1 v2 -> j <= i -> V j v1 v2) ->
+    forall i j {vs1 vs2},
+      Forall2 (V i) vs1 vs2 ->
+      j <= i ->
+      Forall2 (V j) vs1 vs2.
+  Proof.
+    intros V_mono. intros.
+    revert j H0.
+    induction H; simpl; intros; auto.
+    constructor; eauto.
+  Qed.
 
-  (* Analysis result specification *)
-  Parameter analysis_spec : web_map -> A0.exp -> Prop.
+  Definition V_ex0 (v1 : A0.val) (v2 : A1.val) : Prop :=
+    match v1, v2 with
+    | A0.Vconstr t1 vs1, A1.Vconstr t2 vs2 => t1 = t2 /\ length vs1 = length vs2
+    | A0.Vfun f1 ρ1 xs1 e1, A1.Vfun f2 ρ2 xs2 e2 => length xs1 = length xs2
+    | _, _ => False
+    end.
 
-  (* For any Annotate pass, it should produce at least one exposed web ids *)
-  Parameter Exposed_nonempty : exists w, w \in Exposed.
+  Definition V_ex
+    (V' : nat -> A0.val -> A1.wval -> Prop)
+    (E' : nat -> A0.env -> A0.exp -> A1.env -> A1.exp -> Prop)
+    (i0 : nat) (v1 : A0.val) (w2 : web) (v2 : A1.val) :=
+    match v1, v2 with
+    | A0.Vconstr t1 vs1, A1.Vconstr t2 vs2 =>
+        t1 = t2 /\
+        Forall2 (V' i0) vs1 vs2
 
-  (* Specification *)
-  Parameter trans : web_map -> vars -> A0.exp -> A1.exp -> Prop.
+    | A0.Vfun f1 ρ1 xs1 e1, A1.Vfun f2 ρ2 xs2 e2 =>
+        length xs1 = length xs2 /\
+        forall j vs1 vs2 ρ3 ρ4,
+          j <= i0 ->
+          Forall exposed vs2 ->
+          Forall2 (V' j) vs1 vs2 ->
+          set_lists xs1 vs1 (M.set f1 (A0.Vfun f1 ρ1 xs1 e1) ρ1) = Some ρ3 ->
+          set_lists xs2 vs2 (M.set f2 (Tag w2 (A1.Vfun f2 ρ2 xs2 e2)) ρ2) = Some ρ4 ->
+          E' j ρ3 e1 ρ4 e2
+    | _, _ => False
+    end.
 
-  (* A successful analysis should always allow us to transform the program *)
-  Parameter trans_total :
-    forall W e1,
-      web_map_inv W ->
-      analysis_spec W e1 ->
-      exists e2,
-        trans W (A0.occurs_free e1) e1 e2.
+  Lemma V_ex_V_ex0 { V E i v1 w2 v2 }:
+    V_ex V E i v1 w2 v2 -> V_ex0 v1 v2.
+  Proof.
+    unfold V_ex, V_ex0.
+    intros.
+    destruct v1; destruct v2; simpl in H; try contradiction.
+    - fcrush.
+    - destruct H as [Hc HF]; subst.
+      split; auto.
+      eapply Forall2_length; eauto.
+  Qed.
 
-  (* `Erase` is left inverse of `trans` *)
-  (* `Erase o Annotate = id` *)
-  Parameter trans_erase :
-    forall W e1 e2 e1',
-      Annotate.trans W (A0.occurs_free e1) e1 e1' ->
-      Erase.trans (A1.occurs_free e1') e1' e2 ->
-      e1 = e2.
+  Definition R' (P : nat -> A0.val -> A1.wval -> Prop) (i : nat) (r1 : A0.res) (r2 : A1.res) :=
+    match r1, r2 with
+    | A0.OOT, A1.OOT => True
+    | A0.Res v1, A1.Res v2 => P i v1 v2
+    | _, _ => False
+    end.
+
+  Definition E' (P : nat -> A0.val -> A1.wval -> Prop) (ex : bool) (i : nat) (ρ1 : A0.env) (e1 :A0.exp) (ρ2 : A1.env) (e2 : A1.exp) : Prop :=
+    forall j1 r1,
+      j1 <= i ->
+      A0.bstep_fuel ρ1 e1 j1 r1 ->
+      exists j2 r2,
+        A1.bstep_fuel ex ρ2 e2 j2 r2 /\
+        R' P (i - j1) r1 r2.
+
+End AnnotateUtil.
+
+Module Type VAnn.
+
+  Parameter V_ann0 : A0.val -> A1.val -> Prop.
+
+  Parameter V_ann : (nat -> A0.val -> A1.wval -> Prop) ->
+                    (bool -> nat -> A0.env -> A0.exp -> A1.env -> A1.exp -> Prop) ->
+                    nat -> A0.val -> web -> A1.val -> Prop.
+
+  Parameter V_ann_V_ann0 :
+    forall V E i v1 w2 v2,
+      V_ann V E i v1 w2 v2 ->
+      V_ann0 v1 v2.
+
+  Parameter V_ann_mono :
+    forall V E i j v1 w2 v2,
+      (forall k : nat,
+          k < S i ->
+          forall (j : nat) (v1 : A0.val) (v2 : A1.wval), V k v1 v2 -> j <= k -> V j v1 v2) ->
+      V_ann (fun i' => V (i - (i - i'))) (fun b i' => E b (i - (i - i'))) i v1 w2 v2 ->
+      j <= i ->
+      V_ann (fun j' => V (j - (j - j'))) (fun b j' => E b (j - (j - j'))) j v1 w2 v2.
+
+End VAnn.
+
+Module AnnotateV (VA : VAnn).
+
+  Import VA.
+  Export AnnotateUtil.
 
   (* Cross-language Logical Relations *)
-  Parameter V : web_map -> nat -> A0.val -> A1.wval -> Prop.
+  Fixpoint V (i : nat) (v1 : A0.val) (wv2 : A1.wval) {struct i} : Prop :=
+    wf_val wv2 /\
+    match wv2 with
+    | A1.TAG _ w2 v2 =>
+        match i with
+        | 0 =>
+            match exposedb w2 with
+            | true => exposed wv2 /\ V_ex0 v1 v2
+            | false => V_ann0 v1 v2
+            end
 
-  Parameter V_wf_val_r :
-    forall W i v1 v2,
-      V W i v1 v2 ->
-      wf_val v2.
+        | S i0 =>
+            let V' := (fun j v1 wv2 => V (i0 - (i0 - j)) v1 wv2) in
+            let E' b := (fun j ρ1 e1 ρ2 e2 => E' V b (i0 - (i0 - j)) ρ1 e1 ρ2 e2) in
+            match exposedb w2 with
+            | true => exposed wv2 /\ V_ex V' (E' true) i0 v1 w2 v2
+            | false => V_ann V' E' i0 v1 w2 v2
+            end
+        end
+    end.
 
-  Parameter R : web_map -> nat -> A0.res -> A1.res -> Prop.
+  Definition R := (R' V).
 
-  Parameter R_res_inv_l :
-    forall W i v1 r2,
-      R W i (A0.Res v1) r2 ->
-      exists v2, r2 = A1.Res v2 /\ V W i v1 v2.
+  Definition E := (E' V).
 
-  (* Top-level Logical Relations *)
-  Parameter G_top : web_map -> nat -> vars -> A0.env -> vars -> A1.env -> Prop.
+  (* Lemmas about [wf_val], [wf_res], and [wf_env] *)
+  Lemma V_wf_val_r {i v1 v2}:
+    V i v1 v2 ->
+    wf_val v2.
+  Proof.
+    intros HV.
+    destruct i; simpl in *;
+      destruct HV as [Hv2 _]; auto.
+  Qed.
 
-  Parameter G_top_wf_env_r :
-    forall W i Γ1 ρ1 Γ2 ρ2,
-      G_top W i Γ1 ρ1 Γ2 ρ2 ->
-      wf_env ρ2.
+  Lemma V_wf_val_Forall_r {i vs1 vs2} :
+    Forall2 (V i) vs1 vs2 ->
+    Forall wf_val vs2.
+  Proof.
+    intros.
+    induction H; auto.
+    constructor; auto.
+    eapply V_wf_val_r; eauto.
+  Qed.
 
-  Parameter G_top_subset :
-    forall W i Γ1 ρ1 Γ2 ρ2 Γ3 Γ4,
-      G_top W i Γ1 ρ1 Γ2 ρ2 ->
-      Γ3 \subset Γ1 ->
-      Γ4 \subset Γ3 ->
-      G_top W i Γ3 ρ1 Γ4 ρ2.
+  Lemma V_wf_res_r {i v1 v2}:
+    V i v1 v2 ->
+    wf_res (Res v2).
+  Proof.
+    intros HV.
+    constructor.
+    eapply V_wf_val_r; eauto.
+  Qed.
 
-  Parameter trans_correct_top : web_map -> A0.exp -> A1.exp -> Prop.
+  Lemma R_wf_res_l {i r1 r2} :
+    R i r1 r2 ->
+    wf_res r2.
+  Proof.
+    unfold R.
+    intros.
+    destruct r1; destruct r2; try contradiction; auto.
+    constructor.
+    eapply V_wf_val_r; eauto.
+  Qed.
 
-  Parameter top :
-    forall W e1 e2,
-      trans W (A0.occurs_free e1) e1 e2 ->
-      trans_correct_top W e1 e2.
+  (* Inversion Lemmas *)
+  Lemma R_res_inv_l i v1 r2 :
+    R i (A0.Res v1) r2 ->
+    exists v2, r2 = A1.Res v2 /\ V i v1 v2.
+  Proof.
+    intros.
+    destruct r2; simpl in *; try contradiction.
+    eexists; split; eauto.
+  Qed.
 
-  Parameter trans_correct_top_subset :
-    forall W e1 e2,
-      trans_correct_top W e1 e2 ->
-      A1.occurs_free e2 \subset A0.occurs_free e1.
+  (* Monotonicity Lemmas *)
+  Lemma V_ex_mono :
+    forall i V E j v1 w2 v2,
+      (forall k : nat,
+          k < S i ->
+          forall (j : nat) (v1 : A0.val) (v2 : wval), V k v1 v2 -> j <= k -> V j v1 v2) ->
+      V_ex (fun i' => V (i - (i - i'))) (fun i' => E (i - (i - i'))) i v1 w2 v2 ->
+      j <= i ->
+      V_ex (fun j' => V (j - (j - j'))) (fun j' => E (j - (j - j'))) j v1 w2 v2.
+  Proof.
+    unfold V_ex.
+    intros.
+    destruct v1; destruct v2; auto;
+      simpl in *; try contradiction.
+    - destruct H0 as [Hlen HV].
+      repeat (split; auto); intros.
+      specialize (HV j0 vs1 vs2 ρ3 ρ4).
+      rewrite normalize_step in *; try lia.
+      eapply HV; eauto; try lia.
+    - destruct H0 as [Heqc HF];
+        repeat split; auto.
+      rewrite normalize_step in *; try lia.
+      eapply V_mono_Forall_aux; eauto; lia.
+  Qed.
+
+  Lemma V_mono i :
+      forall {j v1 v2},
+        V i v1 v2 ->
+        j <= i ->
+        V j v1 v2.
+    Proof.
+      induction i using lt_wf_rec; intros.
+      destruct v2.
+      destruct i; simpl in H0;
+        destruct j; simpl; intros;
+        destruct H0 as [Hv1 HV]; subst.
+      - repeat (split; auto).
+      - inv H1.
+      - repeat (split; auto).
+        destruct (exposed_reflect w).
+        + inv HV; split; auto.
+          eapply V_ex_V_ex0; eauto.
+        + eapply V_ann_V_ann0; eauto.
+      - repeat (split; auto).
+        destruct (exposed_reflect w).
+        + inv HV; split; auto.
+          eapply V_ex_mono; eauto; lia.
+        + eapply V_ann_mono; eauto; lia.
+    Qed.
+
+  Lemma V_mono_Forall i j {vs1 vs2} :
+    Forall2 (V i) vs1 vs2 ->
+    j <= i ->
+    Forall2 (V j) vs1 vs2.
+  Proof.
+    intros.
+    eapply V_mono_Forall_mono; eauto.
+    eapply V_mono; eauto.
+  Qed.
+
+  Lemma R_mono {r1 r2} i j :
+    R i r1 r2 ->
+    j <= i ->
+    R j r1 r2.
+  Proof.
+    unfold R.
+    intros.
+    destruct r1; auto.
+    destruct r2; auto.
+    eapply V_mono; eauto.
+  Qed.
+
+  Lemma E_mono {ex ρ1 ρ2 e1 e2} i j:
+    E ex i ρ1 e1 ρ2 e2 ->
+    j <= i ->
+    E ex j ρ1 e1 ρ2 e2.
+  Proof.
+    unfold E, R, E', R'.
+    intros.
+    destruct (H j1 r1) as [j2 [r2 [Hr2 HR]]]; auto; try lia.
+    exists j2, r2; split; eauto.
+    apply R_mono with (i - j1); try lia; auto.
+  Qed.
+
+End AnnotateV.
+
+Module AnnotateTop.
+
+  (* The top-level exposed relation is exactly the relation induced by the trivial analysis *)
+  Module VTrivM <: VAnn.
+
+    Definition V_ann0 (v1 : A0.val) (v2 : A1.val) : Prop := False.
+
+    Definition V_ann
+      (V' : nat -> A0.val -> A1.wval -> Prop)
+      (E' : bool -> nat -> A0.env -> A0.exp -> A1.env -> A1.exp -> Prop)
+      (i0 : nat) (v1 : A0.val) (w2 : web) (v2 : A1.val) := False.
+
+    Lemma V_ann_V_ann0 :
+      forall V E i v1 w2 v2,
+        V_ann V E i v1 w2 v2 ->
+        V_ann0 v1 v2.
+    Proof. unfold V_ann, V_ann0; auto. Qed.
+
+    Lemma V_ann_mono V E i j v1 w2 v2 :
+      (forall k : nat,
+          k < S i ->
+          forall (j : nat) (v1 : A0.val) (v2 : A1.wval), V k v1 v2 -> j <= k -> V j v1 v2) ->
+      V_ann (fun i' => V (i - (i - i'))) (fun b i' => E b (i - (i - i'))) i v1 w2 v2 ->
+      j <= i ->
+      V_ann (fun j' => V (j - (j - j'))) (fun b j' => E b (j - (j - j'))) j v1 w2 v2.
+    Proof. unfold V_ann. intros; fcrush. Qed.
+
+  End VTrivM.
+
+  Module VM := AnnotateV VTrivM.
+  Export VM.
+
+  (* Top-level Environment Relation *)
+  Definition G i Γ1 ρ1 Γ2 ρ2 :=
+    wf_env ρ2 /\
+    Γ2 \subset Γ1 /\
+    forall x,
+      (x \in Γ1) ->
+      exists v1 v2,
+        M.get x ρ1 = Some v1 /\
+        M.get x ρ2 = Some v2 /\
+        V i v1 v2.
+
+  Lemma G_wf_env_r i Γ1 ρ1 Γ2 ρ2 :
+    G i Γ1 ρ1 Γ2 ρ2 ->
+    wf_env ρ2.
+  Proof. unfold G. intros; tauto. Qed.
+
+  Lemma G_subset_inv i Γ1 ρ1 Γ2 ρ2 :
+    G i Γ1 ρ1 Γ2 ρ2 ->
+    Γ2 \subset Γ1.
+  Proof. unfold G; intros; tauto. Qed.
+
+  Lemma G_subset i Γ1 ρ1 Γ2 ρ2 Γ3 Γ4 :
+    G i Γ1 ρ1 Γ2 ρ2 ->
+    Γ3 \subset Γ1 ->
+    Γ4 \subset Γ3 ->
+    G i Γ3 ρ1 Γ4 ρ2.
+  Proof.
+    unfold G.
+    intros.
+    destruct H as [Hr [Hs HG]].
+    repeat (split; auto).
+  Qed.
+
+  (* Top-level Monotonicity Lemma *)
+  Lemma G_mono {Γ1 Γ2 ρ1 ρ2} i j:
+      G i Γ1 ρ1 Γ2 ρ2 ->
+      j <= i ->
+      G j Γ1 ρ1 Γ2 ρ2.
+  Proof.
+    unfold G.
+    intros.
+    destruct H as [Hwf [HS HG]].
+    split; auto.
+    split; auto; intros.
+    edestruct HG as [v1 [v2 [Heqv1 [Heqv2 HV]]]]; eauto.
+    eexists; eexists; repeat (split; eauto).
+    apply V_mono with i; eauto.
+  Qed.
+
+  (* Top-level Relation *)
+  Definition trans_correct etop etop' :=
+    A1.occurs_free etop' \subset A0.occurs_free etop /\
+    forall i ρ1 ρ2,
+      G i (A0.occurs_free etop) ρ1 (A1.occurs_free etop') ρ2 ->
+      E true i ρ1 etop ρ2 etop'.
+
+  Lemma trans_correct_subset e1 e2 :
+    trans_correct e1 e2 ->
+    A1.occurs_free e2 \subset A0.occurs_free e1.
+  Proof.
+    unfold trans_correct.
+    intros.
+    inv H; auto.
+  Qed.
+
+  (* Cross-language Compositionality *)
 
   (* Adequacy *)
-  Parameter adequacy :
-    forall W e1 e2,
-      web_map_inv W ->
-      trans_correct_top W e1 e2 ->
-      forall ρ1 ρ2,
-        wf_env ρ2 ->
-        (forall k, G_top W k (A0.occurs_free e1) ρ1 (A1.occurs_free e2) ρ2) ->
-        forall j1 r1,
-          A0.bstep_fuel ρ1 e1 j1 r1 ->
-          exists j2 r2,
-            A1.bstep_fuel true ρ2 e2 j2 r2 /\
-            (forall k, R W k r1 r2).
+  Theorem adequacy e1 e2:
+    trans_correct e1 e2 ->
+    forall ρ1 ρ2,
+      wf_env ρ2 ->
+      (forall k, G k (A0.occurs_free e1) ρ1 (A1.occurs_free e2) ρ2) ->
+      forall j1 r1,
+        A0.bstep_fuel ρ1 e1 j1 r1 ->
+        exists j2 r2,
+          A1.bstep_fuel true ρ2 e2 j2 r2 /\
+          (forall k, R k r1 r2).
+  Proof.
+    intros.
+    unfold trans_correct in H.
+    destruct H as [HS HT].
+
+    assert (HE : E true j1 ρ1 e1 ρ2 e2) by (eapply (HT j1); eauto).
+    edestruct (HE j1) as [j2 [r2 [Hstep2 HR]]]; eauto.
+    eexists; eexists; split; eauto.
+
+    intros.
+    assert (HE' : E true (j1 + k) ρ1 e1 ρ2 e2) by (eapply HT; eauto).
+    edestruct (HE' j1) as [j2' [r2' [Hstep2' HR']]]; eauto; try lia.
+
+    rewrite_math (j1 + k - j1 = k).
+    rewrite_math (j1 - j1 = 0).
+
+    destruct r2; destruct r2'; destruct r1;
+      simpl in *; auto; try contradiction.
+
+    edestruct (A1.bstep_fuel_deterministic w w0 Hstep2 Hstep2'); subst; eauto.
+  Qed.
 
   (* Behavioral Refinement *)
-  Parameter val_ref : A0.val -> A1.wval -> Prop.
+  Inductive val_ref_ : A0.val -> A1.wval -> Prop :=
+  | Ref_Vfun :
+    forall f1 ρ1 w xs1 e1 f2 ρ2 xs2 e2,
+      val_ref_ (A0.Vfun f1 ρ1 xs1 e1) (Tag w (A1.Vfun f2 ρ2 xs2 e2))
 
-  Parameter V_val_ref :
-    forall W v1 v2,
-      (forall i, V W i v1 v2) ->
+  | Ref_Vconstr_nil :
+    forall w c,
+      val_ref_ (A0.Vconstr c []) (Tag w (A1.Vconstr c []))
+
+  | Ref_Vconstr_cons :
+    forall w c v1 v2 vs1 vs2,
+      val_ref_ v1 v2 ->
+      val_ref_ (A0.Vconstr c vs1) (Tag w (A1.Vconstr c vs2)) ->
+      val_ref_ (A0.Vconstr c (v1 :: vs1)) (Tag w (A1.Vconstr c (v2 :: vs2))).
+
+  Hint Constructors val_ref_ : core.
+
+  Definition val_ref := val_ref_.
+
+  Hint Unfold val_ref : core.
+
+  Lemma val_ref_Vconstr c w vs1 vs2 :
+    Forall2 val_ref vs1 vs2 ->
+    val_ref (A0.Vconstr c vs1) (Tag w (A1.Vconstr c vs2)).
+  Proof.
+    intros.
+    induction H; simpl; auto.
+  Qed.
+
+  Theorem V_val_ref {v1 v2} :
+    (forall i, V i v1 v2) ->
+    val_ref v1 v2.
+    Proof.
+      unfold val_ref.
+      revert v2.
+      induction v1 using val_ind'; intros; simpl.
+      - specialize (H 0).
+        destruct v2.
+        simpl in H.
+        destruct H as [Hwf HV].
+        destruct (exposed_reflect w); inv HV.
+        destruct v; try contradiction.
+        inv H0.
+        destruct l; try discriminate; auto.
+      - destruct v2.
+        pose proof (H 0) as H0; simpl in *.
+        destruct H0 as [Hw HV].
+        destruct (exposed_reflect w); inv HV.
+        destruct v; try contradiction.
+        destruct H1 as [Hc Hlen]; subst.
+
+        destruct l0; simpl in *; inv Hlen.
+        inv H0.
+
+        assert (HV' : forall i, V i v1 t /\ V i (A0.Vconstr c l) (Tag w (A1.Vconstr c l0))).
+        {
+          intros.
+          specialize (H (S i0)); simpl in *.
+          destruct H as [_ HV]; subst.
+          destruct (exposed_reflect w); try contradiction.
+          destruct HV as [Hex [Hc HFV]]; subst; eauto.
+
+          inv HFV.
+          split.
+          eapply V_mono; eauto; lia.
+
+          assert (He' : exposed (Tag w (A1.Vconstr c l0))).
+          {
+            inv Hex; inv H6; auto.
+          }
+
+          assert (Hw' : wf_val (Tag w (A1.Vconstr c l0))).
+          {
+            constructor; intros; auto.
+            inv Hw.
+            inv H5; auto.
+          }
+
+          inv H6.
+          inv Hw.
+          inv H8.
+          destruct i0; simpl in *;
+            destruct (exposed_reflect w); try contradiction;
+            repeat (split; auto);
+            simpl in *;
+            rewrite_math (i0 - i0 = 0);
+            rewrite_math (i0 - 0 = i0);
+            try (eapply V_mono_Forall; eauto; lia).
+        }
+
+        assert (HV0 : forall i, V i v1 t) by (intros i0; destruct (HV' i0); auto).
+        assert (HV1 : forall i, V i (A0.Vconstr c l) (Tag w (A1.Vconstr c l0))) by (intros i0; destruct (HV' i0); auto).
+        auto.
+      - specialize (H 0); simpl in *.
+        destruct H as [Hw HV].
+        destruct v2; try contradiction; auto.
+        destruct (exposed_reflect w); inv HV.
+        destruct v; try contradiction; auto.
+    Qed.
+
+    Corollary R_res_val_ref {v1 v2} :
+      (forall i, R i (A0.Res v1) (A1.Res v2)) ->
       val_ref v1 v2.
+    Proof. intros; eapply V_val_ref; eauto. Qed.
 
-  Parameter R_res_val_ref :
-    forall W v1 v2,
-      (forall i, R W i (A0.Res v1) (A1.Res v2)) ->
-      val_ref v1 v2.
 
-  (* Preconditions for linking *)
-  Parameter linking_inv : web_map -> var -> var -> Prop.
-
-  (* Linking Preservation *)
-  Parameter preserves_linking :
-    forall W f w x e1 e2 e1' e2',
-      linking_inv W f x ->
-      (w \in Exposed) ->
-      trans_correct_top W e1 e2 ->
-      trans_correct_top W e1' e2' ->
-      trans_correct_top W (A0.link f x e1 e1') (A1.link f w x e2 e2').
-
-End Annotate.
+End AnnotateTop.
